src/cbor/spec/raw/CBOR.Spec.API.Format.fst
@@ -47,3 +47,34 @@ let cbor_det_serialize_tag_correct tag payload =
   R.mk_det_raw_cbor_mk_cbor (R.Tagged (RF.mk_raw_uint64 tag) (R.mk_det_raw_cbor payload));
   assert (R.mk_det_raw_cbor (pack (CTagged tag payload)) == R.Tagged (RF.mk_raw_uint64 tag) (R.mk_det_raw_cbor payload));
   RF.serialize_cbor_tag_correct (RF.mk_raw_uint64 tag) (R.mk_det_raw_cbor payload)
+
+let rec list_map_mk_det_raw_cbor_correct
+  (l: list cbor)
+: Lemma
+  (ensures (
+    let l' = List.Tot.map R.mk_det_raw_cbor l in
+    List.Tot.for_all R.raw_data_item_ints_optimal l' /\
+    List.Tot.for_all (R.raw_data_item_sorted R.deterministically_encoded_cbor_map_key_order) l'
+  ))
+= match l with
+  | [] -> ()
+  | _ :: q -> list_map_mk_det_raw_cbor_correct q
+
+let rec list_map_mk_cbor_mk_det_raw_cbor
+  (l: list cbor)
+: Lemma
+  (ensures (
+    List.Tot.map R.mk_cbor (List.Tot.map R.mk_det_raw_cbor l) == l
+  ))
+= match l with
+  | [] -> ()
+  | _ :: q -> list_map_mk_cbor_mk_det_raw_cbor q
+
+let cbor_det_serialize_list l =
+  R.serialize_cbor_list (List.Tot.map R.mk_det_raw_cbor l)
+
+let cbor_det_serialize_list_nil () =
+  R.serialize_cbor_list_nil ()
+
+let cbor_det_serialize_list_cons a q =
+  R.serialize_cbor_list_cons (R.mk_det_raw_cbor a) (List.Tot.map R.mk_det_raw_cbor q)
